src/reflection/FStar.Reflection.Basic.fsti
@@ -35,7 +35,7 @@ val lookup_attr           : term -> Env.env -> list fv
 val all_defs_in_env       : Env.env -> list fv
 val defs_in_module        : Env.env -> name -> list fv
 val binders_of_env        : Env.env -> binders
-val vars_of_env           : Env.env -> list bv
+val vars_of_env           : Env.env -> list RD.binding
 val moduleof              : Env.env -> list string
 val term_eq               : term -> term -> bool
 val env_open_modules      : Env.env -> list name
